Directory Pointer

app/src/main/dafny/eventSet.dfy
@@ -3,28 +3,28 @@ class Event{
 }
 
 datatype EventSet=EventSet(events: set<Event>){
-  static function empty(): EventSet {
+  static function Empty(): EventSet {
     EventSet({})
   }
 
-  method add() returns (r: EventSet)
-    ensures isBefore(r)
+  method Add() returns (r: EventSet)
+    ensures IsBefore(r)
     ensures fresh(r.events - events)
   {
     var e := new Event();
     r := EventSet(events + {e});
   }
 
-  function merge(other: EventSet): EventSet {
+  function Merge(other: EventSet): EventSet {
     EventSet(events + other.events)
   }
 
-  predicate isBefore(other: EventSet){
+  predicate IsBefore(other: EventSet){
     this!=other && forall e :: e in events ==> e in other.events
   }
 
-  predicate isConcurrent(other: EventSet){
-    !this.isBefore(other) && !other.isBefore(this)
+  predicate IsConcurrent(other: EventSet){
+    !this.IsBefore(other) && !other.IsBefore(this)
   }
 }
 
