app/src/main/dafny/eventSetTests.dfy
@@ -2,27 +2,27 @@ include "eventSet.dfy"
 include "vectorClock.dfy"
 
 method testBasics(){
-  var a:= EventSet.empty();
-  var b:=a.add();
-  var c:=a.add();
-  var d:=b.merge(c);
-  assert b.isConcurrent(c);
-  assert a.isBefore(b);
-  assert b.isBefore(d);
-  assert c.isBefore(d);
+  var a:= EventSet.Empty();
+  var b:=a.Add();
+  var c:=a.Add();
+  var d:=b.Merge(c);
+  assert b.IsConcurrent(c);
+  assert a.IsBefore(b);
+  assert b.IsBefore(d);
+  assert c.IsBefore(d);
 }
 
 method testEquivalence(){
-  var a:=EventSet.empty();
+  var a:=EventSet.Empty();
   var ac:=VectorClock.empty();
 
-  var b:=a.add();
+  var b:=a.Add();
   var bc:=ac.inc(1);
 
-  var c:=a.add();
+  var c:=a.Add();
   var cc:=ac.inc(2);
 
-  assert a.isBefore(b)== ac.isBefore(bc);
-  assert a.isBefore(c)== ac.isBefore(cc);
-  assert b.isBefore(c)== bc.isBefore(cc);
+  assert a.IsBefore(b)== ac.isBefore(bc);
+  assert a.IsBefore(c)== ac.isBefore(cc);
+  assert b.IsBefore(c)== bc.isBefore(cc);
 }
