app/src/main/dafny/treeTest.dfy
@@ -1,0 +1,96 @@
+module TreeTest {
+
+  datatype Tree<T> =
+      Node(left: Tree<T>, right: Tree<T>)
+    | Leaf(value: T)
+  {
+    function  pointer(): Pointer<T> {
+      Pointer(Root, this)
+    }
+  }
+
+  // A location identifies a subtree by recording the path from the root.
+  datatype Location<T> =
+      Root
+    | Left(parent: Location<T>, right: Tree<T>)
+    | Right(parent: Location<T>, left: Tree<T>)
+  {
+    // Reconstruct the whole tree by placing t at this location.
+    function  reconstruct(t: Tree<T>): Tree<T>
+    {
+      match this
+      case Root =>
+        t
+      case Left(parent, right) =>
+        parent.reconstruct(Node(t, right))
+      case Right(parent, left) =>
+        parent.reconstruct(Node(left, t))
+    }
+
+    // Construct the immediate parent subtree containing t.
+    function  parentTree(t: Tree<T>): Tree<T>
+    {
+      match this
+      case Root =>
+        t
+      case Left(_, right) =>
+        Node(t, right)
+      case Right(_, left) =>
+        Node(left, t)
+    }
+  }
+
+  // A pointer identifies a subtree together with its location in the tree.
+  datatype Pointer<T> = Pointer(
+    location: Location<T>,
+    subtree: Tree<T>
+  )
+  {
+    function left(): (result: Pointer<T>)
+      requires subtree.Node?
+      ensures result.reconstruct() == reconstruct()
+    {
+      Pointer(Left(location, subtree.right), subtree.left)
+    }
+
+    function right(): (result: Pointer<T>)
+      requires subtree.Node?
+      ensures result.reconstruct() == reconstruct()
+    {
+      Pointer(Right(location, subtree.left), subtree.right)
+    }
+
+    function parent(): (result:Pointer<T>)
+      requires location != Root
+      ensures result.reconstruct() == reconstruct()
+    {
+      Pointer(location.parent, location.parentTree(subtree))
+    }
+
+    function replace(newSubtree: Tree<T>): (result: Pointer<T>)
+    {
+      Pointer(location, newSubtree)
+    }
+
+    function reconstruct(): Tree<T>
+    {
+      location.reconstruct(subtree)
+    }
+  }
+
+  method testOperations()
+  {
+    var tree := Node(Leaf(0), Leaf(1));
+    var pointer := tree.pointer();
+
+    assert pointer.left().subtree.value == 0;
+    assert pointer.right().subtree.value == 1;
+
+    assert pointer.left().reconstruct() == tree;
+    assert pointer.left().parent() == pointer;
+
+    assert pointer.right().replace(Leaf(2)).reconstruct()
+        == Node(Leaf(0), Leaf(2));
+  }
+
+}
